lean/src/r_correct_theorem.lean
@@ -1,12 +1,184 @@
+import tactic
+import .a_eval_theorem
+
 import .defs
 variable [GuardModule]
 open GuardModule
+
+local attribute [simp] ant_eval'._match_2
+
+lemma foo (tr1: Ant Φ) (tr2: Ant Φ) (env: Env):
+    ant_eval (tr1.branch tr2) env
+    = ant_eval'._match_1 (ant_eval tr1 env) (ant_eval tr2 env) :=
+begin
+    simp [ant_eval, ant_eval_all, map_ant, ant_eval'],
+end
+
+lemma foo_1 (tr: Ant Φ) (ty: Φ) (env: Env):
+    ant_eval (Ant.diverge ty tr) env
+    = ant_eval'._match_2 (Φ_eval ty env) (ant_eval tr env) :=
+begin
+    simp [ant_eval, ant_eval_all, map_ant, ant_eval'],
+end
+
+lemma ant_eval_branch (tr1: Ant Φ) (tr2: Ant Φ) (env: Env) (r: Result)
+    (h: ant_eval (tr1.branch tr2) env = some r):
+        ant_eval tr1 env = some r ∨ ant_eval tr2 env = some r :=
+begin
+    rw foo at h,
+    cases ant_eval tr1 env with val1;
+    try { cases val1, };
+    cases ant_eval tr2 env with val2;
+    try { cases val2, };
+    finish
+end
+
+lemma ant_eval_diverge { ty: Φ } { tr: Ant Φ } { env: Env } { r: Result }
+    (h: ant_eval (Ant.diverge ty tr) env = some r):
+        Φ_eval ty env == ff ∧ ant_eval tr env = some r
+        ∨ Φ_eval ty env == tt ∧ r = Result.diverged :=
+begin
+    rw foo_1 at h,
+    cases Φ_eval ty env;
+    cases ant_eval tr env with val;
+    try { cases val, };
+    finish,
+end
+
+def ℛ'_diverge (a: list Leaf) (i: list Leaf) (r: list Leaf) (is_empty: bool) (ant: Ant bool)
+    (h1: ℛ' ant = (a, i, r)):
+    (is_empty = false ∧ a = [] ∧ i = []  ∧ ∃ rh: Leaf, ∃ rs: list Leaf, r = rh::rs ∧ ℛ' (Ant.diverge is_empty ant) = ([], [rh], rs))
+    ∨ ((is_empty = true ∨ a ≠ [] ∨ i ≠ [] ∨ r = []) ∧ ℛ' (Ant.diverge is_empty ant) = (a, i, r)) :=
+begin
+    cases is_empty;
+    cases a;
+    cases i;
+    cases r;
+    simp [ℛ', ℛ'._match_1, h1],
+end
+
+-- (a, i, r) = ℛ is_empty.val (Ant.diverge ant_a ant_tr)
+
+def ℛ'_diverge' (ty: Φ) (tr: Ant Φ) (): sorry := sorry
+
+lemma r_correct_1 [decidable_eq Leaf]
+    (is_empty: Gs) (gdt: Gdt)
+    
+    (ant: Ant Φ)
+    (h1: ant_eval ant = some ∘ gdt_eval gdt)
+
+    (a: list Leaf) (i: list Leaf) (r: list Leaf)
+    (h2: (a, i, r) = ℛ is_empty.val ant)
+    
+    (env: Env) (leaf: Leaf)
+    (h3: gdt_eval gdt env = Result.leaf leaf):
+
+        leaf ∈ a
+
+    :=
+begin
+    replace h3: ant_eval ant env = some(Result.leaf leaf), sorry, -- finish
+    clear h1,
+    
+    induction ant generalizing a i r env,
+
+    case Ant.branch {
+        sorry,
+        /-
+        rw ℛ at h2,
+        rw map_ant at h2,
+        rw ℛ' at h2,
+        rw ←ℛ at h2,
+        rw ←ℛ at h2,
+
+        replace h3 := ant_eval_branch h3,
+
+        cases ℛ is_empty.val ant_tr1 with tr1_a tr1_,
+        cases tr1_ with tr1_i tr1_r,
+
+        cases ℛ is_empty.val ant_tr2 with tr2_a tr2_,
+        cases tr2_ with tr2_i tr2_r,
+
+
+        rw ℛ'._match_2 at h2,
+
+        cases h3,
+
+        case or.inl {
+            have: leaf ∈ tr1_a := begin
+                specialize ant_ih_tr1 tr1_a tr1_i tr1_r env,
+                simp at ant_ih_tr1,
+                rw h3 at ant_ih_tr1,
+                simp at ant_ih_tr1,
+                exact ant_ih_tr1,
+            end,
+            finish,
+        },
+
+        case or.inr {
+            have: leaf ∈ tr2_a := begin
+                specialize ant_ih_tr2 tr2_a tr2_i tr2_r env,
+                simp at ant_ih_tr2,
+                rw h3 at ant_ih_tr2,
+                simp at ant_ih_tr2,
+                exact ant_ih_tr2,
+            end,
+            finish,
+        },
+        -/
+    },
+
+    case Ant.diverge {
+        rw ℛ at h2,
+        rw map_ant at h2,
+        rw ℛ' at h2,
+        rw ←ℛ at h2,
+
+        replace h3 := ant_eval_diverge h3,
+        cases ℛ is_empty.val ant_tr with tr_a tr_,
+        cases tr_ with tr_i tr_r,
+
+        have x := ℛ'_diverge a i r (is_empty.val ant_a) (map_ant is_empty.val ant_tr),
+        rw ℛ at h2,
+        rw h2 at x,
+
+        rw ℛ'._match_1 at h2,
+    },
+end
+
+
+#print prefix ℛ'._match_1
+
+
+
+
+
+
+
+
+
+
+
+
+
+
+
+
+
+
+
+
+
+
+
+
 
 -- Every redundant leaf can be marked as inaccessible instead and
 -- every inaccessible leaf can be marked as accessible instead without invalidating the theorem. This only weakens the analysis.
 
 theorem r_correct [decidable_eq Leaf] : ∀ gdt: Gdt, ∀ is_empty: Gs,
     (
+        -- structure + später matchen
         let ⟨ a, i, r ⟩ := ℛ is_empty.val $ 𝒜 gdt
         in
                 -- Leaves that are redundant and neither accessible nor inaccessible can be removed without changing semantics.
@@ -27,5 +199,7 @@ theorem r_correct [decidable_eq Leaf] : ∀ gdt: Gdt, ∀ is_empty: Gs,
         : Prop
     )
     -- We probably need 𝒜_eval for proving this.
-    := sorry
-
+    :=
+begin
+    
+end
